theories/Factor_Transaction_Values.thy
@@ -8,6 +8,24 @@ definition snapshot_value_presents :: "selection_snapshot \<Rightarrow> factor_t
   "snapshot_value_presents S t \<longleftrightarrow> snapshot_formed S \<and>
     data_collection_presents generation_value_presents (fset S) t"
 
+theorem snapshot_value_presentation_class:
+  "presentation_class snapshot_value_presents snapshot_formed (\<lambda>t. \<exists>S. snapshot_value_presents S t)"
+proof -
+  have raw: "presentation_class (data_fset_presents generation_value_presents)
+      (\<lambda>S. \<forall>G\<in>fset S. generation_formed G)
+      (presented_predicate (data_sequence_presents generation_value_presents) distinct)"
+    by (rule data_fset_presentation_class[OF generation_value_presentation_class])
+  have restricted: "presentation_class
+      (\<lambda>S t. snapshot_formed S \<and> data_fset_presents generation_value_presents S t)
+      snapshot_formed (\<lambda>t. \<exists>S. snapshot_formed S \<and> data_fset_presents generation_value_presents S t)"
+    by (rule presentation_class_subdomain[OF raw]) (simp add: snapshot_formed_def selection_formed_def)
+  show ?thesis using restricted by (simp only: presentation_class_def snapshot_value_presents_def)
+qed
+
+interpretation snapshot_values: presentation_class snapshot_value_presents snapshot_formed
+  "\<lambda>t. \<exists>S. snapshot_value_presents S t"
+  by (rule snapshot_value_presentation_class)
+
 lemma snapshot_value_presents_formed:
   assumes present: "snapshot_value_presents S t"
   shows "snapshot_formed S \<and> term_formed t \<and> self_contained_term t"
@@ -24,27 +42,20 @@ qed
 lemma snapshot_value_presents_unique:
   assumes first: "snapshot_value_presents S t" and second: "snapshot_value_presents U t"
   shows "S=U"
-proof -
-  have left: "data_collection_presents generation_value_presents (fset S) t"
-    and right: "data_collection_presents generation_value_presents (fset U) t"
-    using first second by (auto simp: snapshot_value_presents_def)
-  have "fset S=fset U" by (rule data_collection_presents_unique[OF left right])
-    (rule generation_value_presents_unique; assumption)
-  then show ?thesis by (simp add: fset_inject)
-qed
+  by (rule snapshot_values.recovery[OF first second])
 
 theorem snapshot_value_presents_total:
   assumes formed: "snapshot_formed S"
   shows "\<exists>t. snapshot_value_presents S t"
-proof -
-  have cores: "\<forall>G\<in>fset S. generation_formed G"
-    using formed by (simp add: snapshot_formed_def selection_formed_def)
-  have each: "\<forall>G\<in>fset S. \<exists>t. generation_value_presents G t"
-    using cores generation_value_presents_total by blast
-  obtain t where "data_collection_presents generation_value_presents (fset S) t"
-    using data_collection_presents_total[OF finite_fset each] by blast
-  then show ?thesis using formed unfolding snapshot_value_presents_def by blast
-qed
+  by (rule snapshot_values.total[OF formed])
+
+theorem snapshot_quotation_presentation_class:
+  "presentation_class
+    (composed_presentation snapshot_value_presents (\<lambda>t p. complete_data_quoted_at (fst p) (snd p) t))
+    snapshot_formed
+    (\<lambda>p. \<exists>t. (\<exists>S. snapshot_value_presents S t) \<and> complete_data_quoted_at (fst p) (snd p) t)"
+  by (rule complete_quotation_presentation_class[OF snapshot_value_presentation_class])
+    (use snapshot_value_presents_formed in blast)
 
 section \<open>The four independent transaction fields as ordinary data\<close>
 
@@ -56,39 +67,49 @@ definition transaction_value_presents :: "structural_transaction \<Rightarrow> f
       data_collection_presents target_value_presents (fset (proposed_absent T)) d \<and>
       t=Pair_Term a (Pair_Term b (Pair_Term c d)))"
 
+theorem transaction_value_presentation_class:
+  "presentation_class transaction_value_presents transaction_formed
+    (\<lambda>t. \<exists>T. transaction_value_presents T t)"
+proof -
+  let ?S="\<lambda>t. \<exists>U. snapshot_value_presents U t"
+  let ?T="presented_predicate (data_sequence_presents target_value_presents) distinct"
+  let ?tail="\<lambda>t. \<exists>p q. ?S p \<and> ?T q \<and> t=Pair_Term p q"
+  let ?middle="\<lambda>t. \<exists>p q. ?T p \<and> ?tail q \<and> t=Pair_Term p q"
+  let ?A="\<lambda>t. \<exists>p q. ?S p \<and> ?middle q \<and> t=Pair_Term p q"
+  let ?R="factor_pair_presents snapshot_value_presents
+    (factor_pair_presents (data_fset_presents target_value_presents)
+      (factor_pair_presents snapshot_value_presents (data_fset_presents target_value_presents)))"
+  let ?D="\<lambda>z. snapshot_formed (fst z) \<and>
+    ((\<forall>x\<in>fset (fst (snd z)). target_formed x) \<and>
+      (snapshot_formed (fst (snd (snd z))) \<and> (\<forall>x\<in>fset (snd (snd (snd z))). target_formed x)))"
+  have fields: "presentation_class ?R ?D ?A"
+    by (rule factor_pair_class[OF snapshot_value_presentation_class
+      factor_pair_class[OF data_fset_presentation_class[OF target_value_presentation_class]
+        factor_pair_class[OF snapshot_value_presentation_class
+          data_fset_presentation_class[OF target_value_presentation_class]]]])
+  let ?observe="\<lambda>T. (expected_selected T,(expected_absent T,(proposed_selected T,proposed_absent T)))"
+  have observed: "presentation_class (\<lambda>T t. transaction_formed T \<and> ?R (?observe T) t)
+      transaction_formed (\<lambda>t. \<exists>T. transaction_formed T \<and> ?R (?observe T) t)"
+  proof (rule presentation_class_observations[OF fields])
+    fix T assume "transaction_formed T"
+    then show "?D (?observe T)" by (simp add: transaction_formed_def)
+  next
+    fix T U assume "transaction_formed T" "transaction_formed U" "?observe T=?observe U"
+    then show "T=U" by (simp add: structural_transaction_identity)
+  qed
+  have reading: "(transaction_formed T \<and> ?R (?observe T) t) \<longleftrightarrow> transaction_value_presents T t" for T t
+    by (auto simp: transaction_value_presents_def factor_pair_presents_def; blast)
+  show ?thesis using observed by (simp only: reading)
+qed
+
+interpretation transaction_values: presentation_class transaction_value_presents transaction_formed
+  "\<lambda>t. \<exists>T. transaction_value_presents T t"
+  by (rule transaction_value_presentation_class)
+
 theorem transaction_value_presents_unique:
   assumes first: "transaction_value_presents S t" and second: "transaction_value_presents T t"
   shows "S=T"
-proof -
-  obtain a b c d where left: "snapshot_value_presents (expected_selected S) a"
-    "data_collection_presents target_value_presents (fset (expected_absent S)) b"
-    "snapshot_value_presents (proposed_selected S) c"
-    "data_collection_presents target_value_presents (fset (proposed_absent S)) d"
-    "t=Pair_Term a (Pair_Term b (Pair_Term c d))"
-    using first unfolding transaction_value_presents_def by blast
-  obtain a' b' c' d' where right: "snapshot_value_presents (expected_selected T) a'"
-    "data_collection_presents target_value_presents (fset (expected_absent T)) b'"
-    "snapshot_value_presents (proposed_selected T) c'"
-    "data_collection_presents target_value_presents (fset (proposed_absent T)) d'"
-    "t=Pair_Term a' (Pair_Term b' (Pair_Term c' d'))"
-    using second unfolding transaction_value_presents_def by blast
-  have same: "a'=a" "b'=b" "c'=c" "d'=d" using left(5) right(5) by simp_all
-  have other: "snapshot_value_presents (expected_selected T) a"
-    "data_collection_presents target_value_presents (fset (expected_absent T)) b"
-    "snapshot_value_presents (proposed_selected T) c"
-    "data_collection_presents target_value_presents (fset (proposed_absent T)) d"
-    using right(1-4) same by simp_all
-  have selected: "expected_selected S=expected_selected T" "proposed_selected S=proposed_selected T"
-    by (rule snapshot_value_presents_unique[OF left(1) other(1)])
-       (rule snapshot_value_presents_unique[OF left(3) other(3)])
-  have absent: "fset (expected_absent S)=fset (expected_absent T)"
-    by (rule data_collection_presents_unique[OF left(2) other(2)])
-       (rule target_value_presents_unique; assumption)
-  have removed: "fset (proposed_absent S)=fset (proposed_absent T)"
-    by (rule data_collection_presents_unique[OF left(4) other(4)])
-       (rule target_value_presents_unique; assumption)
-  show ?thesis using selected absent removed by (simp add: structural_transaction_identity fset_inject)
-qed
+  by (rule transaction_values.recovery[OF first second])
 
 lemma transaction_value_presents_formed:
   assumes present: "transaction_value_presents T t"
@@ -116,24 +137,15 @@ qed
 theorem transaction_value_presents_total:
   assumes formed: "transaction_formed T"
   shows "\<exists>t. transaction_value_presents T t"
-proof -
-  have sf: "snapshot_formed (expected_selected T)" "snapshot_formed (proposed_selected T)"
-    and absent: "\<forall>l\<in>fset (expected_absent T). target_formed l"
-    and removed: "\<forall>l\<in>fset (proposed_absent T). target_formed l"
-    using formed by (auto simp: transaction_formed_def)
-  obtain a c where snapshots: "snapshot_value_presents (expected_selected T) a"
-    "snapshot_value_presents (proposed_selected T) c"
-    using snapshot_value_presents_total[OF sf(1)] snapshot_value_presents_total[OF sf(2)] by blast
-  have each_absent: "\<forall>l\<in>fset (expected_absent T). \<exists>v. target_value_presents l v"
-    using absent target_value_presents_total by blast
-  have each_removed: "\<forall>l\<in>fset (proposed_absent T). \<exists>v. target_value_presents l v"
-    using removed target_value_presents_total by blast
-  obtain b where expected: "data_collection_presents target_value_presents (fset (expected_absent T)) b"
-    using data_collection_presents_total[OF finite_fset each_absent] by blast
-  obtain d where proposed: "data_collection_presents target_value_presents (fset (proposed_absent T)) d"
-    using data_collection_presents_total[OF finite_fset each_removed] by blast
-  show ?thesis using formed snapshots expected proposed unfolding transaction_value_presents_def by blast
-qed
+  by (rule transaction_values.total[OF formed])
+
+theorem transaction_quotation_presentation_class:
+  "presentation_class
+    (composed_presentation transaction_value_presents (\<lambda>t p. complete_data_quoted_at (fst p) (snd p) t))
+    transaction_formed
+    (\<lambda>p. \<exists>t. (\<exists>T. transaction_value_presents T t) \<and> complete_data_quoted_at (fst p) (snd p) t)"
+  by (rule complete_quotation_presentation_class[OF transaction_value_presentation_class])
+    (use transaction_value_presents_formed in blast)
 
 theorem transaction_value_quotation_total:
   assumes "transaction_formed T"
@@ -146,6 +158,69 @@ proof -
   show ?thesis using present complete_data_quotation_total[OF formed closed] by blast
 qed
 
+section \<open>The complete supplied context determines the transaction outcome\<close>
+
+abbreviation transaction_context_presents ::
+  "(selection_snapshot\<times>structural_transaction) \<Rightarrow> factor_term \<Rightarrow> bool" where
+  "transaction_context_presents z t \<equiv> factor_pair_presents snapshot_value_presents transaction_value_presents z t"
+
+definition transaction_execution_presents ::
+  "((selection_snapshot\<times>structural_transaction)\<times>transaction_result) \<Rightarrow> factor_term \<Rightarrow> bool" where
+  "transaction_execution_presents z t \<longleftrightarrow> transaction_context_presents (fst z) t \<and>
+    transact (fst (fst z)) (snd (fst z)) (snd z)"
+
+theorem transaction_execution_presentation_class:
+  "presentation_class transaction_execution_presents
+    (\<lambda>z. transact (fst (fst z)) (snd (fst z)) (snd z))
+    (\<lambda>t. \<exists>z. transaction_context_presents z t)"
+proof -
+  let ?D="\<lambda>z. snapshot_formed (fst z) \<and> transaction_formed (snd z)"
+  let ?A="\<lambda>t. \<exists>p q. (\<exists>S. snapshot_value_presents S p) \<and>
+    (\<exists>T. transaction_value_presents T q) \<and> t=Pair_Term p q"
+  interpret inputs: presentation_class transaction_context_presents ?D ?A
+    by (rule factor_pair_class[OF snapshot_value_presentation_class transaction_value_presentation_class])
+  have determined: "transact (fst z) (snd z) x \<Longrightarrow> transact (fst z) (snd z) y \<Longrightarrow> x=y" for z x y
+    by (rule transaction_result_determined)
+  have result: "presentation_class
+      (\<lambda>z t. transaction_context_presents (fst z) t \<and> transact (fst (fst z)) (snd (fst z)) (snd z))
+      (\<lambda>z. ?D (fst z) \<and> transact (fst (fst z)) (snd (fst z)) (snd z))
+      (\<lambda>t. \<exists>z out. transaction_context_presents z t \<and> transact (fst z) (snd z) out)"
+    by (rule presentation_class_determined[OF inputs.presentation_class_axioms determined])
+  have domain: "(?D (fst z) \<and> transact (fst (fst z)) (snd (fst z)) (snd z)) \<longleftrightarrow>
+      transact (fst (fst z)) (snd (fst z)) (snd z)" for z
+    by (auto simp: transact_def)
+  have admission: "(\<exists>z out. transaction_context_presents z t \<and> transact (fst z) (snd z) out) \<longleftrightarrow>
+      (\<exists>z. transaction_context_presents z t)" for t
+    using inputs.subject_boundary transaction_result_exists by blast
+  show ?thesis using result by (simp only: presentation_class_def transaction_execution_presents_def domain admission)
+qed
+
+theorem transaction_execution_presented_outcome:
+  assumes presented: "transaction_execution_presents ((S,T),out) t"
+  shows "transact S T out"
+    and "out=Applied U \<longrightarrow> comparison_passes S T \<and> U=transaction_update S T \<and>
+      (\<forall>l. snapshot_lookup U l =
+        (if l\<in>snapshot_loci (proposed_selected T) then snapshot_lookup (proposed_selected T) l
+         else if l\<in>fset (proposed_absent T) then None else snapshot_lookup S l))"
+    and "out=Conflict C \<longrightarrow> \<not>comparison_passes S T \<and>
+      C=observed_comparison S T \<and> rel_dom C=comparison_loci T \<and>
+      (\<forall>l\<in>comparison_loci T. (l,snapshot_lookup S l)\<in>C) \<and> finite C \<and>
+      transaction_output out=None"
+proof -
+  have actual: "transact S T out" using presented by (simp add: transaction_execution_presents_def)
+  show "transact S T out" by (rule actual)
+  show "out=Applied U \<longrightarrow> comparison_passes S T \<and> U=transaction_update S T \<and>
+      (\<forall>l. snapshot_lookup U l =
+        (if l\<in>snapshot_loci (proposed_selected T) then snapshot_lookup (proposed_selected T) l
+         else if l\<in>fset (proposed_absent T) then None else snapshot_lookup S l))"
+    using actual successful_transaction_lookup by (auto simp: transact_applied_iff)
+  show "out=Conflict C \<longrightarrow> \<not>comparison_passes S T \<and>
+      C=observed_comparison S T \<and> rel_dom C=comparison_loci T \<and>
+      (\<forall>l\<in>comparison_loci T. (l,snapshot_lookup S l)\<in>C) \<and> finite C \<and>
+      transaction_output out=None"
+    using actual conflict_contains_every_observation by (auto simp: transact_conflict_iff)
+qed
+
 text \<open>
   Snapshot data contains every exact selected core, including its recursive
   history. Transaction data keeps expected selections, expected absence,
@@ -153,6 +228,17 @@ text \<open>
   finite collection admits every complete presentation. Equal presented data
   recovers the exact source fields, without asserting comparison success,
   continuation permission, cause validity, or authority.
+
+  The value classes use the general finite-set, product, subdomain, and
+  observation constructions. The original snapshot and transaction formation
+  conditions remain their independent domains. Complete quotations use the
+  same composition rule.
+
+  Together with the supplied initial snapshot, these fields also determine
+  the whole execution result. Its class recovers a successful update or the
+  complete failed comparison, including every observed locus and value. No
+  outcome field is added to the supplied transaction, and no conflict is
+  presented as a partially applied update.
 \<close>
 
 end
