theories/Factor_Generation_Presentations.thy
@@ -1,0 +1,894 @@
+theory Factor_Generation_Presentations
+  imports Factor_Generation_Values Factor_Judgment_Presentations RRA_Generation_Construction
+begin
+
+section \<open>The actual source context determines the complete generation\<close>
+
+type_synonym generation_source = "site_context\<times>generation_core"
+type_synonym generation_predecessor_row =
+  "local_address\<times>(local_address\<times>(local_address option definition_site\<times>generation_core))"
+
+abbreviation generation_at_context :: "site_context \<Rightarrow> generation_core \<Rightarrow> bool" where
+  "generation_at_context z G \<equiv> generation_at (fst z) (fst (snd z)) (snd (snd z)) G"
+
+lemma generation_context_formed:
+  assumes "generation_at E u r G"
+  shows "environment_formed E \<and> (u,r)\<in>environment_positions E"
+  using generation_at_environment_formed[OF assms] generation_at_has_anchor[OF assms]
+  by (auto simp: anchor_formed_def)
+
+definition generation_source_presents :: "generation_source \<Rightarrow> factor_term \<Rightarrow> bool" where
+  "generation_source_presents z t \<longleftrightarrow>
+    source_root_presents (fst z) t \<and> generation_at_context (fst z) (snd z)"
+
+theorem generation_source_presentation_class:
+  "presentation_class generation_source_presents
+    (\<lambda>z. generation_at_context (fst z) (snd z))
+    (\<lambda>t. \<exists>z. generation_source_presents z t)"
+proof -
+  have unique: "generation_at_context z G \<Longrightarrow> generation_at_context z H \<Longrightarrow> G=H" for z G H
+    by (rule generation_at_unique)
+  have determined: "presentation_class
+      (\<lambda>z t. source_root_presents (fst z) t \<and> generation_at_context (fst z) (snd z))
+      (\<lambda>z. site_context_formed (fst z) \<and> generation_at_context (fst z) (snd z))
+      (\<lambda>t. \<exists>z G. source_root_presents z t \<and> generation_at_context z G)"
+    by (rule presentation_class_determined[OF source_root_presentation_class unique])
+  have formed: "site_context_formed z" if read: "generation_at_context z G" for z G
+    using generation_context_formed[OF read] by simp
+  have domain: "(site_context_formed z \<and> generation_at_context z G) \<longleftrightarrow> generation_at_context z G" for z G
+    using formed by blast
+  have admission: "(\<exists>z G. source_root_presents z t \<and> generation_at_context z G) \<longleftrightarrow>
+      (\<exists>z. generation_source_presents z t)" for t
+    by (auto simp: generation_source_presents_def; metis fst_conv snd_conv)
+  show ?thesis using determined
+    by (simp only: presentation_class_def generation_source_presents_def domain admission)
+qed
+
+interpretation generation_sources: presentation_class generation_source_presents
+  "\<lambda>z. generation_at_context (fst z) (snd z)" "\<lambda>t. \<exists>z. generation_source_presents z t"
+  by (rule generation_source_presentation_class)
+
+lemma generation_source_presents_formed:
+  assumes presented: "generation_source_presents z t"
+  shows "term_formed t \<and> self_contained_term t"
+proof -
+  obtain E u r G where shape: "z=((E,(u,r)),G)"
+    by (rule that[of "fst (fst z)" "fst (snd (fst z))" "snd (snd (fst z))" "snd z"]) simp
+  have source: "source_root_presents (E,(u,r)) t"
+    using presented shape by (simp add: generation_source_presents_def)
+  show ?thesis by (rule source_root_presents_formed[OF source])
+qed
+
+theorem generation_source_presentation_total:
+  assumes source: "generation_at E u r G"
+  shows "\<exists>t. generation_source_presents ((E,(u,r)),G) t \<and> term_formed t \<and> self_contained_term t"
+proof -
+  have domain: "generation_at_context (fst ((E,(u,r)),G)) (snd ((E,(u,r)),G))" using source by simp
+  obtain t where presented: "generation_source_presents ((E,(u,r)),G) t"
+    using generation_sources.total[OF domain] by blast
+  show ?thesis using presented generation_source_presents_formed[OF presented] by blast
+qed
+
+definition generation_core_source_presents :: "generation_core \<Rightarrow> factor_term \<Rightarrow> bool" where
+  "generation_core_source_presents G t \<longleftrightarrow> (\<exists>z. generation_source_presents z t \<and> snd z=G)"
+
+theorem generation_core_source_presentation_class:
+  "presentation_class generation_core_source_presents generation_formed
+    (\<lambda>t. \<exists>z. generation_source_presents z t)"
+proof -
+  have projected: "presentation_class (\<lambda>G t. \<exists>z. generation_source_presents z t \<and> snd z=G)
+      generation_formed (\<lambda>t. \<exists>z. generation_source_presents z t)"
+  proof (rule presentation_class_image[OF generation_source_presentation_class])
+    fix z assume "generation_at_context (fst z) (snd z)"
+    then show "generation_formed (snd z)" by (rule generation_at_formed)
+  next
+    fix G assume "generation_formed G"
+    then obtain E :: "local_address option artifact_environment" and u where read: "generation_at E u [] G"
+      using generation_presentation_total by blast
+    show "\<exists>z. generation_at_context (fst z) (snd z) \<and> snd z=G"
+      by (rule exI[of _ "((E,(u,[])),G)"]) (use read in simp)
+  qed
+  show ?thesis using projected by (simp only: presentation_class_def generation_core_source_presents_def)
+qed
+
+theorem generation_source_quotation_presentation_class:
+  "presentation_class
+    (composed_presentation generation_source_presents (\<lambda>t p. complete_data_quoted_at (fst p) (snd p) t))
+    (\<lambda>z. generation_at_context (fst z) (snd z))
+    (\<lambda>p. \<exists>t. (\<exists>z. generation_source_presents z t) \<and> complete_data_quoted_at (fst p) (snd p) t)"
+  by (rule complete_quotation_presentation_class[OF generation_source_presentation_class])
+    (use generation_source_presents_formed in blast)
+
+section \<open>A report must present the core read from its actual source\<close>
+
+definition generation_report_presents :: "generation_source \<Rightarrow> factor_term \<Rightarrow> bool" where
+  "generation_report_presents z t \<longleftrightarrow> generation_at_context (fst z) (snd z) \<and>
+    factor_pair_presents source_root_presents generation_value_presents z t"
+
+theorem generation_report_presentation_class:
+  "presentation_class generation_report_presents (\<lambda>z. generation_at_context (fst z) (snd z))
+    (\<lambda>t. \<exists>z. generation_report_presents z t)"
+proof -
+  let ?D="\<lambda>z. site_context_formed (fst z) \<and> generation_formed (snd z)"
+  let ?A="\<lambda>t. \<exists>p q. (\<exists>z. source_root_presents z p) \<and>
+    (\<exists>G. generation_value_presents G q) \<and> t=Pair_Term p q"
+  have raw: "presentation_class (factor_pair_presents source_root_presents generation_value_presents) ?D ?A"
+    by (rule factor_pair_class[OF source_root_presentation_class generation_value_presentation_class])
+  have restricted: "presentation_class
+      (\<lambda>z t. generation_at_context (fst z) (snd z) \<and>
+        factor_pair_presents source_root_presents generation_value_presents z t)
+      (\<lambda>z. generation_at_context (fst z) (snd z))
+      (\<lambda>t. \<exists>z. generation_at_context (fst z) (snd z) \<and>
+        factor_pair_presents source_root_presents generation_value_presents z t)"
+  proof (rule presentation_class_subdomain[OF raw])
+    fix z assume actual: "generation_at_context (fst z) (snd z)"
+    show "?D z" using generation_context_formed[OF actual] generation_at_formed[OF actual] by simp
+  qed
+  show ?thesis using restricted by (simp only: presentation_class_def generation_report_presents_def)
+qed
+
+theorem generation_report_relation:
+  "(\<exists>z. generation_report_presents z (Pair_Term p q)) \<longleftrightarrow>
+    presented_relation source_root_presents generation_value_presents generation_at_context p q"
+  by (auto simp: generation_report_presents_def factor_pair_presents_def presented_relation_def;
+    metis fst_conv snd_conv)
+
+corollary generation_report_at_presentations:
+  assumes context_value: "source_root_presents z p" and core_value: "generation_value_presents G q"
+  shows "(\<exists>w. generation_report_presents w (Pair_Term p q)) \<longleftrightarrow> generation_at_context z G"
+  by (simp only: generation_report_relation
+    presented_relation_at[OF source_root_presentation_class generation_value_presentation_class assms])
+
+lemma generation_report_presents_formed:
+  assumes "generation_report_presents z t"
+  shows "term_formed t \<and> self_contained_term t"
+proof -
+  obtain p q where shape: "t=Pair_Term p q"
+    and fields: "source_root_presents (fst z) p" "generation_value_presents (snd z) q"
+    using assms by (auto simp: generation_report_presents_def factor_pair_presents_def)
+  obtain E u r where source_shape: "fst z=(E,(u,r))"
+    by (rule that[of "fst (fst z)" "fst (snd (fst z))" "snd (snd (fst z))"]) simp
+  have source: "source_root_presents (E,(u,r)) p" using fields(1) source_shape by simp
+  show ?thesis using source_root_presents_formed[OF source]
+    generation_value_presents_formed[OF fields(2)] shape by simp
+qed
+
+theorem generation_report_quotation_presentation_class:
+  "presentation_class
+    (composed_presentation generation_report_presents (\<lambda>t p. complete_data_quoted_at (fst p) (snd p) t))
+    (\<lambda>z. generation_at_context (fst z) (snd z))
+    (\<lambda>p. \<exists>t. (\<exists>z. generation_report_presents z t) \<and> complete_data_quoted_at (fst p) (snd p) t)"
+  by (rule complete_quotation_presentation_class[OF generation_report_presentation_class])
+    (use generation_report_presents_formed in blast)
+
+theorem generation_presented_fields:
+  assumes "generation_source_presents ((E,(u,r)),G) t"
+  shows "\<exists>R lr M payr cr. artifact_at E u R \<and> generation_syntax_at R r lr M payr cr \<and>
+    anchored_at E u lr (generation_locus G) \<and>
+    anchored_at E u payr (generation_payload G) \<and> anchored_at E u cr (generation_cause G)"
+proof -
+  have source: "generation_at E u r G" using assms by (simp add: generation_source_presents_def)
+  obtain l M p c g where fields: "generation_fields_at E u r l M p c"
+    and core: "G=Generation l (Abs_fset (image g (rel_dom M))) p c"
+    using source by (cases rule: generation_at.cases) blast
+  show ?thesis using generation_fields_syntax[OF fields] core by (auto; blast)
+qed
+
+section \<open>Every predecessor row retains its actual socket and cited site\<close>
+
+definition generation_predecessor_rows ::
+  "'u artifact_environment \<Rightarrow> 'u \<Rightarrow> local_address \<Rightarrow>
+    (local_address\<times>(local_address\<times>(('u\<times>local_address)\<times>generation_core))) set" where
+  "generation_predecessor_rows E u r =
+    {(s,(d,(z,H))). \<exists>l M p c. generation_fields_at E u r l M p c \<and>
+      (s,d)\<in>M \<and> located_at E u d (fst z) (snd z) \<and>
+      generation_at E (fst z) (snd z) H}"
+
+lemma generation_predecessor_rows_at_fields:
+  assumes fields: "generation_fields_at E u r l M p c"
+    and assigned: "\<forall>s d. (s,d)\<in>M \<longrightarrow>
+      (\<exists>v a. located_at E u d v a \<and> generation_at E v a (g s))"
+  shows "(s,(d,(z,H)))\<in>generation_predecessor_rows E u r \<longleftrightarrow>
+    (s,d)\<in>M \<and> located_at E u d (fst z) (snd z) \<and> H=g s"
+proof -
+  have ef: "environment_formed E" using generation_fields_formed[OF fields] by blast
+  show ?thesis
+  proof
+    assume member: "(s,(d,(z,H)))\<in>generation_predecessor_rows E u r"
+    obtain l' M' p' c' where other: "generation_fields_at E u r l' M' p' c'"
+      and parts: "(s,d)\<in>M'" "located_at E u d (fst z) (snd z)"
+        "generation_at E (fst z) (snd z) H"
+      using member by (auto simp: generation_predecessor_rows_def)
+    have same: "M=M'" using generation_fields_unique[OF fields other] by blast
+    have edge: "(s,d)\<in>M" using parts(1) same by simp
+    obtain v a where loc: "located_at E u d v a" and read: "generation_at E v a (g s)"
+      using assigned edge by blast
+    have site: "fst z=v \<and> snd z=a" by (rule located_at_unique[OF ef parts(2) loc])
+    have child: "generation_at E (fst z) (snd z) (g s)" using read site by simp
+    have core: "H=g s" by (rule generation_at_unique[OF parts(3) child])
+    show "(s,d)\<in>M \<and> located_at E u d (fst z) (snd z) \<and> H=g s"
+      using edge parts(2) core by blast
+  next
+    assume parts: "(s,d)\<in>M \<and> located_at E u d (fst z) (snd z) \<and> H=g s"
+    obtain v a where loc: "located_at E u d v a" and read: "generation_at E v a (g s)"
+      using assigned parts by blast
+    have site: "fst z=v \<and> snd z=a" by (rule located_at_unique[OF ef conjunct1[OF conjunct2[OF parts]] loc])
+    have child: "generation_at E (fst z) (snd z) H" using read site parts by simp
+    show "(s,(d,(z,H)))\<in>generation_predecessor_rows E u r"
+      using fields parts child by (auto simp: generation_predecessor_rows_def)
+  qed
+qed
+
+lemma generation_predecessor_rows_fields:
+  assumes fields: "generation_fields_at E u r l M p c"
+    and assigned: "\<forall>s d. (s,d)\<in>M \<longrightarrow>
+      (\<exists>v a. located_at E u d v a \<and> generation_at E v a (g s))"
+  shows "rel_dom (generation_predecessor_rows E u r)=rel_dom M"
+    and "single_valued (generation_predecessor_rows E u r)"
+    and "finite (generation_predecessor_rows E u r)"
+proof -
+  let ?L="generation_predecessor_rows E u r"
+  have ef: "environment_formed E" and finite: "finite M"
+    using generation_fields_formed[OF fields] by blast+
+  have functional: "single_valued M" using fields
+    by (auto simp: generation_fields_at_def family_at_def)
+  have entries: "(s,(d,(z,H)))\<in>?L \<longleftrightarrow>
+      (s,d)\<in>M \<and> located_at E u d (fst z) (snd z) \<and> H=g s" for s d z H
+    by (rule generation_predecessor_rows_at_fields[OF fields assigned])
+  have domain: "rel_dom ?L=rel_dom M"
+  proof (rule set_eqI)
+    fix s
+    show "s\<in>rel_dom ?L \<longleftrightarrow> s\<in>rel_dom M"
+    proof
+      assume "s\<in>rel_dom ?L"
+      then obtain d z H where "(s,(d,(z,H)))\<in>?L" by (auto simp: rel_dom_def)
+      then show "s\<in>rel_dom M" by (auto simp: entries rel_dom_def)
+    next
+      assume "s\<in>rel_dom M"
+      then obtain d where edge: "(s,d)\<in>M" by (auto simp: rel_dom_def)
+      obtain v a where loc: "located_at E u d v a" using assigned edge by blast
+      have "(s,(d,((v,a),g s)))\<in>?L" using edge loc by (simp only: entries fst_conv snd_conv; blast)
+      then show "s\<in>rel_dom ?L" by (auto simp: rel_dom_def)
+    qed
+  qed
+  have unique: "single_valued ?L"
+  proof (unfold single_valued_def, intro allI impI)
+    fix s x y assume both: "(s,x)\<in>?L" "(s,y)\<in>?L"
+    obtain d z H where x: "x=(d,(z,H))"
+      by (rule that[of "fst x" "fst (snd x)" "snd (snd x)"]) simp
+    obtain e w K where y: "y=(e,(w,K))"
+      by (rule that[of "fst y" "fst (snd y)" "snd (snd y)"]) simp
+    have left: "(s,d)\<in>M" "located_at E u d (fst z) (snd z)" "H=g s"
+      and right: "(s,e)\<in>M" "located_at E u e (fst w) (snd w)" "K=g s"
+      using both x y by (auto simp: entries)
+    have endpoints: "d=e" using functional left(1) right(1) by (auto simp: single_valued_def)
+    have other: "located_at E u d (fst w) (snd w)" using right(2) endpoints by simp
+    have coordinates: "fst z=fst w \<and> snd z=snd w"
+      by (rule located_at_unique[OF ef left(2) other])
+    have sites: "z=w" using coordinates by (simp add: prod_eq_iff)
+    show "x=y" using x y endpoints sites left(3) right(3) by simp
+  qed
+  show "rel_dom ?L=rel_dom M" by (rule domain)
+  show "single_valued ?L" by (rule unique)
+  have finite_domain: "finite (rel_dom ?L)" using finite_rel_dom[OF finite] domain by simp
+  show "finite ?L" by (rule finite_single_valued[OF finite_domain unique])
+qed
+
+theorem generation_predecessor_rows_complete:
+  assumes source: "generation_at E u r G"
+  shows "finite (generation_predecessor_rows E u r)"
+    and "single_valued (generation_predecessor_rows E u r)"
+    and "bij_betw (\<lambda>row. snd (snd (snd row))) (generation_predecessor_rows E u r)
+      (fset (generation_predecessors G))"
+proof -
+  obtain l M p c g where fields: "generation_fields_at E u r l M p c"
+    and injective: "inj_on g (rel_dom M)"
+    and assigned: "\<forall>s d. (s,d)\<in>M \<longrightarrow>
+      (\<exists>v a. located_at E u d v a \<and> generation_at E v a (g s))"
+    and core: "G=Generation l (Abs_fset (image g (rel_dom M))) p c"
+    using source by (cases rule: generation_at.cases) blast
+  let ?L="generation_predecessor_rows E u r"
+  let ?last="\<lambda>row. snd (snd (snd row))"
+  have functional: "single_valued ?L" and finite: "finite ?L"
+    using generation_predecessor_rows_fields(2,3)[OF fields assigned] by blast+
+  have entries: "(s,(d,(z,H)))\<in>?L \<longleftrightarrow>
+      (s,d)\<in>M \<and> located_at E u d (fst z) (snd z) \<and> H=g s" for s d z H
+    by (rule generation_predecessor_rows_at_fields[OF fields assigned])
+  have finite_image: "finite (image g (rel_dom M))"
+    using generation_fields_formed[OF fields] finite_rel_dom by blast
+  have predecessors: "fset (generation_predecessors G)=image g (rel_dom M)"
+    using finite_image by (simp add: core Abs_fset_inverse)
+  have range: "image ?last ?L=image g (rel_dom M)"
+  proof (rule set_eqI)
+    fix H
+    show "H\<in>image ?last ?L \<longleftrightarrow> H\<in>image g (rel_dom M)"
+    proof
+      assume "H\<in>image ?last ?L"
+      then obtain row where member: "row\<in>?L" and core_value: "H=?last row" by blast
+      obtain s d z K where shape: "row=(s,(d,(z,K)))"
+        by (rule that[of "fst row" "fst (snd row)" "fst (snd (snd row))" "snd (snd (snd row))"]) simp
+      have edge: "(s,d)\<in>M" and child: "K=g s" using member shape by (auto simp: entries)
+      show "H\<in>image g (rel_dom M)" using edge child core_value shape by (auto simp: rel_dom_def)
+    next
+      assume "H\<in>image g (rel_dom M)"
+      then obtain s d where edge: "(s,d)\<in>M" and child: "H=g s" by (auto simp: rel_dom_def)
+      obtain v a where loc: "located_at E u d v a" using assigned edge by blast
+      have member: "(s,(d,((v,a),H)))\<in>?L" using edge loc child by (simp only: entries fst_conv snd_conv; blast)
+      show "H\<in>image ?last ?L" by (rule image_eqI[where x="(s,(d,((v,a),H)))"]) (use member in auto)
+    qed
+  qed
+  have distinct: "inj_on ?last ?L"
+  proof (rule inj_onI)
+    fix x y assume members: "x\<in>?L" "y\<in>?L" and same: "?last x=?last y"
+    obtain s d z H where x: "x=(s,(d,(z,H)))"
+      by (rule that[of "fst x" "fst (snd x)" "fst (snd (snd x))" "snd (snd (snd x))"]) simp
+    obtain a e w K where y: "y=(a,(e,(w,K)))"
+      by (rule that[of "fst y" "fst (snd y)" "fst (snd (snd y))" "snd (snd (snd y))"]) simp
+    have left: "(s,d)\<in>M" "H=g s" and right: "(a,e)\<in>M" "K=g a"
+      using members x y by (auto simp: entries)
+    have keys: "s=a" using injective left right same x y by (auto simp: inj_on_def rel_dom_def)
+    have one: "(s,(d,(z,H)))\<in>?L" using members(1) x by simp
+    have two: "(s,(e,(w,K)))\<in>?L" using members(2) y keys by simp
+    have same_row: "(d,(z,H))=(e,(w,K))"
+      by (rule single_valued_outputs[OF functional one two])
+    show "x=y" using x y keys same_row by simp
+  qed
+  show "finite ?L" by (rule finite)
+  show "single_valued ?L" by (rule functional)
+  show "bij_betw ?last ?L (fset (generation_predecessors G))"
+    using distinct range predecessors by (simp only: bij_betw_def)
+qed
+
+lemma generation_predecessor_row_reads:
+  assumes "(s,(d,(z,H)))\<in>generation_predecessor_rows E u r"
+  shows "located_at E u d (fst z) (snd z) \<and> generation_at E (fst z) (snd z) H"
+  using assms by (auto simp: generation_predecessor_rows_def)
+
+corollary generation_predecessor_rows_recover_members:
+  assumes source: "generation_at E u r G"
+  shows "H\<in>fset (generation_predecessors G) \<longleftrightarrow>
+    (\<exists>s d z. (s,(d,(z,H)))\<in>generation_predecessor_rows E u r)"
+proof -
+  let ?L="generation_predecessor_rows E u r"
+  let ?last="\<lambda>row. snd (snd (snd row))"
+  have range: "fset (generation_predecessors G)=image ?last ?L"
+    using generation_predecessor_rows_complete(3)[OF source]
+    by (simp only: bij_betw_def; blast)
+  show ?thesis
+  proof
+    assume member: "H\<in>fset (generation_predecessors G)"
+    have in_image: "H\<in>image ?last ?L" using member by (simp only: range)
+    obtain row where child: "H=?last row" and row: "row\<in>?L"
+      using in_image by (rule imageE)
+    have shape: "row=(fst row,(fst (snd row),(fst (snd (snd row)),H)))"
+      using child by (simp add: prod_eq_iff)
+    have complete: "(fst row,(fst (snd row),(fst (snd (snd row)),H)))\<in>?L"
+      using row by (simp only: shape[symmetric])
+    show "\<exists>s d z. (s,(d,(z,H)))\<in>?L"
+      by (rule exI[of _ "fst row"], rule exI[of _ "fst (snd row)"],
+        rule exI[of _ "fst (snd (snd row))"], rule complete)
+  next
+    assume "\<exists>s d z. (s,(d,(z,H)))\<in>?L"
+    then obtain s d z where row: "(s,(d,(z,H)))\<in>?L" by blast
+    have "H\<in>image ?last ?L"
+      by (rule image_eqI[where x="(s,(d,(z,H)))"]) (use row in auto)
+    then show "H\<in>fset (generation_predecessors G)" using range by simp
+  qed
+qed
+
+theorem generation_predecessor_request_relation:
+  assumes source: "generation_at E u r G"
+  shows "((u,r),(v,a))\<in>generation_request_edges E \<longleftrightarrow>
+    (\<exists>s d H. (s,(d,((v,a),H)))\<in>generation_predecessor_rows E u r)"
+proof -
+  have ef: "environment_formed E" by (rule generation_at_environment_formed[OF source])
+  obtain l M p c g where fields: "generation_fields_at E u r l M p c"
+    and assigned: "\<forall>s d. (s,d)\<in>M \<longrightarrow>
+      (\<exists>w b. located_at E u d w b \<and> generation_at E w b (g s))"
+    using source by (cases rule: generation_at.cases) blast
+  obtain R lr payr cr where art: "artifact_at E u R" and layout: "generation_syntax_at R r lr M payr cr"
+    using generation_fields_syntax[OF fields] by blast
+  have roots: "generation_predecessor_roots R r=rel_ran M"
+    by (rule generation_roots_from_syntax(2)[OF layout])
+  have entries: "(s,(d,(z,H)))\<in>generation_predecessor_rows E u r \<longleftrightarrow>
+      (s,d)\<in>M \<and> located_at E u d (fst z) (snd z) \<and> H=g s" for s d z H
+    by (rule generation_predecessor_rows_at_fields[OF fields assigned])
+  show ?thesis
+  proof
+    assume "((u,r),(v,a))\<in>generation_request_edges E"
+    then obtain S d where other: "artifact_at E u S" "d\<in>generation_predecessor_roots S r"
+      and loc: "located_at E u d v a" by (auto simp: generation_request_edges_def)
+    have same: "R=S" by (rule environment_artifact_unique[OF ef art other(1)])
+    obtain s where edge: "(s,d)\<in>M" using other(2) same roots by (auto simp: rel_ran_def)
+    have "(s,(d,((v,a),g s)))\<in>generation_predecessor_rows E u r"
+      using edge loc by (simp only: entries fst_conv snd_conv; blast)
+    then show "\<exists>s d H. (s,(d,((v,a),H)))\<in>generation_predecessor_rows E u r" by blast
+  next
+    assume "\<exists>s d H. (s,(d,((v,a),H)))\<in>generation_predecessor_rows E u r"
+    then obtain s d H where member: "(s,(d,((v,a),H)))\<in>generation_predecessor_rows E u r" by blast
+    have edge: "(s,d)\<in>M" and loc: "located_at E u d v a" using member by (auto simp: entries)
+    have predecessor: "d\<in>generation_predecessor_roots R r" using edge roots by (auto simp: rel_ran_def)
+    show "((u,r),(v,a))\<in>generation_request_edges E"
+      using art predecessor loc by (auto simp: generation_request_edges_def)
+  qed
+qed
+
+corollary generation_request_decreases_core:
+  assumes parent: "generation_at E u r G" and edge: "((u,r),(v,a))\<in>generation_request_edges E"
+    and child: "generation_at E v a H"
+  shows "H\<in>fset (generation_predecessors G) \<and> size H<size G"
+proof -
+  obtain s d K where row: "(s,(d,((v,a),K)))\<in>generation_predecessor_rows E u r"
+    using edge by (simp only: generation_predecessor_request_relation[OF parent]) blast
+  have read: "generation_at E v a K" using generation_predecessor_row_reads[OF row] by simp
+  have same: "K=H" by (rule generation_at_unique[OF read child])
+  have member: "H\<in>fset (generation_predecessors G)"
+    using row same by (simp only: generation_predecessor_rows_recover_members[OF parent]; blast)
+  have decreased: "size H<size G"
+    by (rule predecessor_size_decreases) (use member in \<open>simp add: predecessor_edges_def\<close>)
+  show ?thesis using member decreased by blast
+qed
+
+theorem generation_read_sites_well_founded:
+  assumes roots: "\<forall>u r. (u,r)\<in>roots \<longrightarrow> (\<exists>G. generation_at E u r G)"
+  shows "wf {(v,u). u\<in>generation_read_sites E roots \<and> (u,v)\<in>generation_request_edges E}"
+proof -
+  let ?core="\<lambda>s. THE G. generation_at E (fst s) (snd s) G"
+  have recovered: "?core s=G" if read: "generation_at E (fst s) (snd s) G" for s G
+  proof (rule the_equality[where P="\<lambda>H. generation_at E (fst s) (snd s) H" and a=G])
+    show "generation_at E (fst s) (snd s) G" by (rule read)
+  next
+    fix H assume other: "generation_at E (fst s) (snd s) H"
+    show "H=G" by (rule generation_at_unique[OF other read])
+  qed
+  have decrease: "{(v,u). u\<in>generation_read_sites E roots \<and> (u,v)\<in>generation_request_edges E}
+      \<subseteq>measure (\<lambda>s. size (?core s))"
+  proof
+    fix edge assume member: "edge\<in>{(v,u). u\<in>generation_read_sites E roots \<and> (u,v)\<in>generation_request_edges E}"
+    obtain u r v a where shape: "edge=((v,a),(u,r))"
+      and site: "(u,r)\<in>generation_read_sites E roots"
+      and link: "((u,r),(v,a))\<in>generation_request_edges E"
+      using member by (auto split: prod.splits)
+    obtain G where parent: "generation_at E u r G" using generation_read_sites_have_cores[OF roots site] by blast
+    obtain H where child: "generation_at E v a H" using generation_request_edge_has_core[OF parent link] by blast
+    have smaller: "size H<size G" using generation_request_decreases_core[OF parent link child] by blast
+    have left: "?core (u,r)=G" and right: "?core (v,a)=H"
+      using recovered[of "(u,r)" G] recovered[of "(v,a)" H] parent child by simp_all
+    show "edge\<in>measure (\<lambda>s. size (?core s))" using shape smaller left right by simp
+  qed
+  show ?thesis by (rule wf_subset[OF wf_measure decrease])
+qed
+
+section \<open>Every successful retained reading preserves the same predecessor rows\<close>
+
+lemma generation_predecessor_rows_included:
+  assumes included: "environment_included F E" and formed: "environment_formed E"
+  shows "generation_predecessor_rows F u r\<subseteq>generation_predecessor_rows E u r"
+proof
+  fix row assume member: "row\<in>generation_predecessor_rows F u r"
+  obtain s d z H where shape: "row=(s,(d,(z,H)))"
+    by (rule that[of "fst row" "fst (snd row)" "fst (snd (snd row))" "snd (snd (snd row))"]) simp
+  obtain l M p c where fields: "generation_fields_at F u r l M p c"
+    and edge: "(s,d)\<in>M" and loc: "located_at F u d (fst z) (snd z)"
+    and child: "generation_at F (fst z) (snd z) H"
+    using member shape by (auto simp: generation_predecessor_rows_def)
+  have larger_fields: "generation_fields_at E u r l M p c"
+    by (rule generation_fields_included[OF included formed fields])
+  have larger_location: "located_at E u d (fst z) (snd z)"
+    by (rule included_located[OF included loc])
+  have larger_child: "generation_at E (fst z) (snd z) H"
+    by (rule generation_at_included[OF child included formed])
+  show "row\<in>generation_predecessor_rows E u r"
+    using larger_fields edge larger_location larger_child
+    by (auto simp: shape generation_predecessor_rows_def)
+qed
+
+theorem generation_predecessor_rows_extension:
+  assumes source: "generation_at F u r G" and included: "environment_included F E"
+    and formed: "environment_formed E"
+  shows "generation_predecessor_rows E u r=generation_predecessor_rows F u r"
+proof -
+  obtain l M p c g where fields: "generation_fields_at F u r l M p c"
+    and assigned: "\<forall>s d. (s,d)\<in>M \<longrightarrow>
+      (\<exists>v a. located_at F u d v a \<and> generation_at F v a (g s))"
+    using source by (cases rule: generation_at.cases) blast
+  have larger: "generation_fields_at E u r l M p c"
+    by (rule generation_fields_included[OF included formed fields])
+  have assignments: "\<forall>s d. (s,d)\<in>M \<longrightarrow>
+      (\<exists>v a. located_at E u d v a \<and> generation_at E v a (g s))"
+    using assigned included formed by (meson included_located generation_at_included)
+  have upper: "generation_predecessor_rows E u r\<subseteq>generation_predecessor_rows F u r"
+  proof
+    fix row assume member: "row\<in>generation_predecessor_rows E u r"
+    obtain s d z H where shape: "row=(s,(d,(z,H)))"
+      by (rule that[of "fst row" "fst (snd row)" "fst (snd (snd row))" "snd (snd (snd row))"]) simp
+    have edge: "(s,d)\<in>M" and loc: "located_at E u d (fst z) (snd z)" and child: "H=g s"
+      using member shape by (auto simp: generation_predecessor_rows_at_fields[OF larger assignments])
+    obtain v a where actual: "located_at F u d v a" "generation_at F v a (g s)" using assigned edge by blast
+    have copied: "located_at E u d v a" by (rule included_located[OF included actual(1)])
+    have site: "fst z=v \<and> snd z=a" by (rule located_at_unique[OF formed loc copied])
+    have location: "located_at F u d (fst z) (snd z)" using actual(1) site by simp
+    show "row\<in>generation_predecessor_rows F u r"
+      using edge location child by (simp only: shape generation_predecessor_rows_at_fields[OF fields assigned]; blast)
+  qed
+  have lower: "generation_predecessor_rows F u r\<subseteq>generation_predecessor_rows E u r"
+    by (rule generation_predecessor_rows_included[OF included formed])
+  show ?thesis using upper lower by blast
+qed
+
+definition generation_source_environment ::
+  "'u artifact_environment \<Rightarrow> 'u \<Rightarrow> local_address \<Rightarrow> 'u artifact_environment" where
+  "generation_source_environment E u r=request_environment E (generation_requests E {(u,r)})"
+
+theorem generation_source_environment_reading:
+  assumes formed: "environment_formed E"
+  shows "generation_at (generation_source_environment E u r) u r G \<longleftrightarrow> generation_at E u r G"
+proof
+  assume read: "generation_at (generation_source_environment E u r) u r G"
+  have included: "environment_included (generation_source_environment E u r) E"
+    by (simp only: generation_source_environment_def) (rule request_environment_included)
+  show "generation_at E u r G" by (rule generation_at_included[OF read included formed])
+next
+  assume read: "generation_at E u r G"
+  have roots: "\<forall>v a. (v,a)\<in>{(u,r)} \<longrightarrow> (\<exists>H. generation_at E v a H)" using read by auto
+  have site: "(u,r)\<in>generation_read_sites E {(u,r)}" using generation_read_sites_roots[of "{(u,r)}" E] by blast
+  show "generation_at (generation_source_environment E u r) u r G"
+    unfolding generation_source_environment_def by (rule generation_at_request_restriction[OF formed roots read site])
+qed
+
+theorem generation_source_environment_properties:
+  assumes source: "generation_at E u r G"
+  shows "environment_formed (generation_source_environment E u r)"
+    and "generation_at (generation_source_environment E u r) u r G"
+    and "generation_environment_closed (generation_source_environment E u r) {(u,r)}"
+    and "generation_read_sites (generation_source_environment E u r) {(u,r)}=generation_read_sites E {(u,r)}"
+    and "generation_requests (generation_source_environment E u r) {(u,r)}=generation_requests E {(u,r)}"
+    and "generation_source_environment (generation_source_environment E u r) u r=generation_source_environment E u r"
+    and "\<forall>v a. (v,a)\<in>generation_read_sites E {(u,r)} \<longrightarrow>
+      generation_predecessor_rows (generation_source_environment E u r) v a=generation_predecessor_rows E v a"
+proof -
+  let ?Q="generation_requests E {(u,r)}"
+  let ?R="generation_source_environment E u r"
+  have ef: "environment_formed E" by (rule generation_at_environment_formed[OF source])
+  have roots: "\<forall>v a. (v,a)\<in>{(u,r)} \<longrightarrow> (\<exists>H. generation_at E v a H)" using source by auto
+  have requests_formed: "citation_requests_formed E ?Q" by (rule generation_requests_formed[OF ef roots])
+  have requests: "generation_requests ?R {(u,r)}=?Q"
+    unfolding generation_source_environment_def by (rule generation_requests_restricted[OF requests_formed])
+  show "environment_formed ?R"
+    unfolding generation_source_environment_def by (rule request_environment_formed[OF requests_formed])
+  show "generation_at ?R u r G" using source by (simp only: generation_source_environment_reading[OF ef])
+  show "generation_environment_closed ?R {(u,r)}"
+    unfolding generation_source_environment_def by (rule generation_closed_restriction[OF ef roots])
+  show "generation_read_sites ?R {(u,r)}=generation_read_sites E {(u,r)}"
+    unfolding generation_source_environment_def by (rule generation_read_sites_restricted[OF requests_formed])
+  show "generation_requests ?R {(u,r)}=?Q" by (rule requests)
+  have once: "generation_source_environment ?R u r=request_environment ?R ?Q"
+    using requests by (simp only: generation_source_environment_def[of ?R u r])
+  have idempotent: "request_environment ?R ?Q=?R"
+    unfolding generation_source_environment_def by (rule request_environment_idempotent)
+  show "generation_source_environment ?R u r=?R" by (rule trans[OF once idempotent])
+  show "\<forall>v a. (v,a)\<in>generation_read_sites E {(u,r)} \<longrightarrow>
+      generation_predecessor_rows ?R v a=generation_predecessor_rows E v a"
+  proof (intro allI impI)
+    fix v a assume site: "(v,a)\<in>generation_read_sites E {(u,r)}"
+    obtain H where read: "generation_at E v a H" using generation_read_sites_have_cores[OF roots site] by blast
+    have retained: "generation_at ?R v a H"
+      unfolding generation_source_environment_def by (rule generation_at_request_restriction[OF ef roots read site])
+    have included: "environment_included ?R E"
+      unfolding generation_source_environment_def by (rule request_environment_included)
+    show "generation_predecessor_rows ?R v a=generation_predecessor_rows E v a"
+      using generation_predecessor_rows_extension[OF retained included ef] by simp
+  qed
+qed
+
+theorem generation_source_environment_least:
+  assumes formed: "environment_formed E" and read: "generation_at F u r H"
+    and included: "environment_included F E"
+  shows "environment_included (generation_source_environment E u r) F"
+proof -
+  have roots: "\<forall>v a. (v,a)\<in>{(u,r)} \<longrightarrow> (\<exists>G. generation_at F v a G)" using read by auto
+  have ff: "environment_formed F" by (rule generation_at_environment_formed[OF read])
+  show ?thesis unfolding generation_source_environment_def
+    by (rule generation_successful_reading_requires_dependencies[OF roots included formed ff])
+qed
+
+theorem generation_source_environment_fixed:
+  assumes closed: "generation_environment_closed E {(u,r)}"
+  shows "generation_source_environment E u r=E"
+proof -
+  let ?Q="generation_requests E {(u,r)}"
+  have uses: "environment_uses E=environment_reachable E {u}"
+    and slots: "rel_dom (environment_bindings E)=requested_slots E ?Q"
+    using closed by (auto simp: generation_environment_closed_def environment_closed_def)
+  obtain G where read: "generation_at E u r G" using closed by (auto simp: generation_environment_closed_def)
+  have site: "(u,r)\<in>generation_read_sites E {(u,r)}" using generation_read_sites_roots[of "{(u,r)}" E] by blast
+  have source: "u\<in>image fst ?Q" by (rule generation_site_has_request[OF read site])
+  have root: "{u}\<subseteq>requested_uses E ?Q" using source by (auto simp: requested_uses_def)
+  have edge_closed: "environment_edge_closed E (requested_uses E ?Q)"
+    using slots by (auto simp: environment_edge_closed_def requested_uses_def rel_dom_def binds_slot_def)
+  have coverage: "environment_uses E\<subseteq>requested_uses E ?Q"
+    using environment_reachable_least[OF root edge_closed] uses by simp
+  show ?thesis unfolding generation_source_environment_def
+    by (rule request_environment_fixed_coverage[OF coverage]) (use slots in simp)
+qed
+
+definition generation_retention_presents ::
+  "(generation_source\<times>local_address option artifact_environment) \<Rightarrow> factor_term \<Rightarrow> bool" where
+  "generation_retention_presents z t \<longleftrightarrow> generation_source_presents (fst z) t \<and>
+    snd z=generation_source_environment (fst (fst (fst z))) (fst (snd (fst (fst z)))) (snd (snd (fst (fst z))))"
+
+theorem generation_retention_presentation_class:
+  "presentation_class generation_retention_presents
+    (\<lambda>z. generation_at_context (fst (fst z)) (snd (fst z)) \<and>
+      snd z=generation_source_environment (fst (fst (fst z))) (fst (snd (fst (fst z)))) (snd (snd (fst (fst z)))))
+    (\<lambda>t. \<exists>z. generation_source_presents z t)"
+proof -
+  let ?scope="\<lambda>z::generation_source.
+    generation_source_environment (fst (fst z)) (fst (snd (fst z))) (snd (snd (fst z)))"
+  have functional: "F=?scope z \<Longrightarrow> H=?scope z \<Longrightarrow> F=H" for z F H by simp
+  have result: "presentation_class (\<lambda>z t. generation_source_presents (fst z) t \<and> snd z=?scope (fst z))
+      (\<lambda>z. generation_at_context (fst (fst z)) (snd (fst z)) \<and> snd z=?scope (fst z))
+      (\<lambda>t. \<exists>z F. generation_source_presents z t \<and> F=?scope z)"
+    by (rule presentation_class_determined[OF generation_source_presentation_class functional])
+  have reading: "generation_retention_presents =
+      (\<lambda>z t. generation_source_presents (fst z) t \<and> snd z=?scope (fst z))"
+    by (rule ext)+ (simp only: generation_retention_presents_def)
+  have admission: "(\<lambda>t. \<exists>z F. generation_source_presents z t \<and> F=?scope z) =
+      (\<lambda>t. \<exists>z. generation_source_presents z t)"
+    by (rule ext) simp
+  show ?thesis using result by (simp only: reading admission)
+qed
+
+theorem generation_presented_retention:
+  assumes presented: "generation_retention_presents (((E,(u,r)),G),F) t"
+  shows "generation_at F u r G"
+    and "generation_environment_closed F {(u,r)}"
+    and "generation_predecessor_rows F u r=generation_predecessor_rows E u r"
+    and "\<forall>v A. artifact_at F v A \<longleftrightarrow> v\<in>requested_uses E (generation_requests E {(u,r)}) \<and> artifact_at E v A"
+    and "\<forall>v s w. binds_slot F v s w \<longleftrightarrow>
+      (v,s)\<in>requested_slots E (generation_requests E {(u,r)}) \<and> binds_slot E v s w"
+proof -
+  have source: "generation_at E u r G" and retained: "F=generation_source_environment E u r"
+    using presented by (auto simp: generation_retention_presents_def generation_source_presents_def)
+  show "generation_at F u r G" "generation_environment_closed F {(u,r)}"
+    using generation_source_environment_properties(2,3)[OF source] retained by auto
+  have site: "(u,r)\<in>generation_read_sites E {(u,r)}" using generation_read_sites_roots[of "{(u,r)}" E] by blast
+  show "generation_predecessor_rows F u r=generation_predecessor_rows E u r"
+    using generation_source_environment_properties(7)[OF source] retained site by blast
+  show "\<forall>v A. artifact_at F v A \<longleftrightarrow> v\<in>requested_uses E (generation_requests E {(u,r)}) \<and> artifact_at E v A"
+    by (simp only: retained generation_source_environment_def artifact_at_request_environment; simp)
+  show "\<forall>v s w. binds_slot F v s w \<longleftrightarrow>
+      (v,s)\<in>requested_slots E (generation_requests E {(u,r)}) \<and> binds_slot E v s w"
+    by (simp only: retained generation_source_environment_def binds_slot_request_environment; simp)
+qed
+
+section \<open>Complete row values preserve every predecessor coordinate\<close>
+
+definition generation_predecessor_row_formed :: "generation_predecessor_row \<Rightarrow> bool" where
+  "generation_predecessor_row_formed row \<longleftrightarrow>
+    octets_formed (fst row) \<and> octets_formed (fst (snd row)) \<and>
+    octets_formed (snd (fst (snd (snd row)))) \<and> generation_formed (snd (snd (snd row)))"
+
+definition generation_predecessor_row_presents :: "generation_predecessor_row \<Rightarrow> factor_term \<Rightarrow> bool" where
+  "generation_predecessor_row_presents row t \<longleftrightarrow> generation_predecessor_row_formed row \<and>
+    factor_pair_presents (\<lambda>a p. p=Payload_Term a)
+      (factor_pair_presents (\<lambda>a p. p=Payload_Term a)
+        (factor_pair_presents site_coordinate_presents generation_value_presents)) row t"
+
+theorem generation_predecessor_row_presentation_class:
+  "presentation_class generation_predecessor_row_presents generation_predecessor_row_formed
+    (\<lambda>t. \<exists>row. generation_predecessor_row_presents row t)"
+proof -
+  let ?P="\<lambda>t. \<exists>a. t=Payload_Term a"
+  let ?S="\<lambda>t. \<exists>z. site_coordinate_presents z t"
+  let ?G="\<lambda>t. \<exists>H. generation_value_presents H t"
+  let ?tail="\<lambda>t. \<exists>p q. ?S p \<and> ?G q \<and> t=Pair_Term p q"
+  let ?middle="\<lambda>t. \<exists>p q. ?P p \<and> ?tail q \<and> t=Pair_Term p q"
+  let ?A="\<lambda>t. \<exists>p q. ?P p \<and> ?middle q \<and> t=Pair_Term p q"
+  let ?R="factor_pair_presents (\<lambda>a p. p=Payload_Term a)
+    (factor_pair_presents (\<lambda>a p. p=Payload_Term a)
+      (factor_pair_presents site_coordinate_presents generation_value_presents))"
+  have raw: "presentation_class ?R (\<lambda>row. generation_formed (snd (snd (snd row)))) ?A"
+    using factor_pair_class[OF address_coordinate_presentation
+      factor_pair_class[OF address_coordinate_presentation
+        factor_pair_class[OF site_coordinate_presentation generation_value_presentation_class]]] by simp
+  have restricted: "presentation_class (\<lambda>row t. generation_predecessor_row_formed row \<and> ?R row t)
+      generation_predecessor_row_formed (\<lambda>t. \<exists>row. generation_predecessor_row_formed row \<and> ?R row t)"
+    by (rule presentation_class_subdomain[OF raw]) (simp add: generation_predecessor_row_formed_def)
+  show ?thesis using restricted by (simp only: presentation_class_def generation_predecessor_row_presents_def)
+qed
+
+lemma generation_predecessor_row_value_formed:
+  assumes presented: "generation_predecessor_row_presents row t"
+  shows "term_formed t \<and> self_contained_term t"
+proof -
+  obtain s d z H where shape: "row=(s,(d,(z,H)))"
+    by (rule that[of "fst row" "fst (snd row)" "fst (snd (snd row))" "snd (snd (snd row))"]) simp
+  obtain v where encoded: "t=Pair_Term (Payload_Term s) (Pair_Term (Payload_Term d)
+      (Pair_Term (site_data_term (fst z) (snd z)) v))"
+    and core: "generation_value_presents H v"
+    using presented shape by (auto simp: generation_predecessor_row_presents_def factor_pair_presents_def)
+  have coordinates: "octets_formed s" "octets_formed d" "octets_formed (snd z)"
+    using presented shape by (auto simp: generation_predecessor_row_presents_def generation_predecessor_row_formed_def)
+  show ?thesis using generation_value_presents_formed[OF core] coordinates encoded by simp
+qed
+
+lemma generation_predecessor_rows_formed:
+  assumes member: "row\<in>generation_predecessor_rows E u r"
+  shows "generation_predecessor_row_formed row"
+proof -
+  obtain s d z H where shape: "row=(s,(d,(z,H)))"
+    by (rule that[of "fst row" "fst (snd row)" "fst (snd (snd row))" "snd (snd (snd row))"]) simp
+  obtain l M p c where fields: "generation_fields_at E u r l M p c"
+    and edge: "(s,d)\<in>M" and child: "generation_at E (fst z) (snd z) H"
+    using member shape by (auto simp: generation_predecessor_rows_def)
+  obtain R pr where formed: "environment_formed E" and art: "artifact_at E u R" and family: "family_at R pr M"
+    using fields by (auto simp: generation_fields_at_def)
+  have exact: "exact_formed R" using formed art by (auto simp: environment_formed_def)
+  have positions: "s\<in>rra_carrier (object_structure R)" "d\<in>rra_carrier (object_structure R)"
+    using family edge by (auto simp: family_at_def headed_incidence_def object_formed_def rra_formed_def)
+  have source_addresses: "octets_formed s" "octets_formed d" using exact positions by (auto simp: exact_formed_def)
+  have site: "z\<in>environment_positions E" using generation_context_formed[OF child] by simp
+  have address: "octets_formed (snd z)" by (rule environment_position_address[OF formed site])
+  have core: "generation_formed H" by (rule generation_at_formed[OF child])
+  show ?thesis using shape source_addresses address core by (simp add: generation_predecessor_row_formed_def)
+qed
+
+interpretation generation_predecessor_collections: presentation_class
+  "data_collection_presents generation_predecessor_row_presents"
+  "\<lambda>L. finite L \<and> (\<forall>row\<in>L. generation_predecessor_row_formed row)"
+  "presented_predicate (data_sequence_presents generation_predecessor_row_presents) distinct"
+  by (rule data_collection_presentation_class[OF generation_predecessor_row_presentation_class])
+
+definition generation_predecessor_report_presents ::
+  "(generation_source\<times>generation_predecessor_row set) \<Rightarrow> factor_term \<Rightarrow> bool" where
+  "generation_predecessor_report_presents z t \<longleftrightarrow>
+    snd z=generation_predecessor_rows (fst (fst (fst z))) (fst (snd (fst (fst z)))) (snd (snd (fst (fst z)))) \<and>
+    factor_pair_presents generation_source_presents
+      (data_collection_presents generation_predecessor_row_presents) z t"
+
+theorem generation_predecessor_report_presentation_class:
+  "presentation_class generation_predecessor_report_presents
+    (\<lambda>z. generation_at_context (fst (fst z)) (snd (fst z)) \<and>
+      snd z=generation_predecessor_rows (fst (fst (fst z))) (fst (snd (fst (fst z)))) (snd (snd (fst (fst z)))))
+    (\<lambda>t. \<exists>z. generation_predecessor_report_presents z t)"
+proof -
+  let ?rows="\<lambda>z::generation_source.
+    generation_predecessor_rows (fst (fst z)) (fst (snd (fst z))) (snd (snd (fst z)))"
+  let ?R="factor_pair_presents generation_source_presents (data_collection_presents generation_predecessor_row_presents)"
+  let ?D="\<lambda>z. generation_at_context (fst (fst z)) (snd (fst z)) \<and> snd z=?rows (fst z)"
+  let ?raw="\<lambda>z. generation_at_context (fst (fst z)) (snd (fst z)) \<and>
+    (finite (snd z) \<and> (\<forall>row\<in>snd z. generation_predecessor_row_formed row))"
+  let ?A="\<lambda>t. \<exists>p q. (\<exists>z. generation_source_presents z p) \<and>
+    presented_predicate (data_sequence_presents generation_predecessor_row_presents) distinct q \<and> t=Pair_Term p q"
+  have fields: "presentation_class ?R ?raw ?A"
+    by (rule factor_pair_class[OF generation_source_presentation_class
+      generation_predecessor_collections.presentation_class_axioms])
+  have restricted: "presentation_class (\<lambda>z t. ?D z \<and> ?R z t) ?D (\<lambda>t. \<exists>z. ?D z \<and> ?R z t)"
+  proof (rule presentation_class_subdomain[OF fields])
+    fix z assume domain: "?D z"
+    have native: "generation_at_context (fst (fst z)) (snd (fst z))" using domain by blast
+    have finite: "finite (?rows (fst z))" by (rule generation_predecessor_rows_complete(1)[OF native])
+    have each: "\<forall>row\<in>?rows (fst z). generation_predecessor_row_formed row"
+      by (blast intro: generation_predecessor_rows_formed)
+    show "?raw z" using domain finite each by simp
+  qed
+  have reading: "(?D z \<and> ?R z t) \<longleftrightarrow> generation_predecessor_report_presents z t" for z t
+    using generation_sources.subject_boundary
+    by (auto simp: generation_predecessor_report_presents_def factor_pair_presents_def)
+  show ?thesis using restricted by (simp only: reading)
+qed
+
+theorem generation_predecessor_report_relation:
+  "(\<exists>z. generation_predecessor_report_presents z (Pair_Term p q)) \<longleftrightarrow>
+    presented_relation generation_source_presents (data_collection_presents generation_predecessor_row_presents)
+      (\<lambda>z L. L=generation_predecessor_rows (fst (fst z)) (fst (snd (fst z))) (snd (snd (fst z)))) p q"
+  by (auto simp: generation_predecessor_report_presents_def factor_pair_presents_def presented_relation_def;
+    metis fst_conv snd_conv)
+
+corollary generation_predecessor_report_at_presentations:
+  assumes source: "generation_source_presents ((E,(u,r)),G) p"
+    and rows: "data_collection_presents generation_predecessor_row_presents L q"
+  shows "(\<exists>z. generation_predecessor_report_presents z (Pair_Term p q)) \<longleftrightarrow>
+    L=generation_predecessor_rows E u r"
+  by (simp only: generation_predecessor_report_relation
+    presented_relation_at[OF generation_source_presentation_class
+      generation_predecessor_collections.presentation_class_axioms assms] fst_conv snd_conv)
+
+lemma generation_predecessor_report_formed:
+  assumes "generation_predecessor_report_presents z t"
+  shows "term_formed t \<and> self_contained_term t"
+proof -
+  obtain p q where source: "generation_source_presents (fst z) p"
+    and rows: "data_collection_presents generation_predecessor_row_presents (snd z) q"
+    and shape: "t=Pair_Term p q"
+    using assms by (auto simp: generation_predecessor_report_presents_def factor_pair_presents_def)
+  have first: "term_formed p \<and> self_contained_term p" by (rule generation_source_presents_formed[OF source])
+  have formed: "term_formed q" by (rule data_collection_presents_formed[OF rows])
+    (use generation_predecessor_row_value_formed in blast)
+  have closed: "self_contained_term q" by (rule data_collection_presents_self_contained[OF rows])
+    (use generation_predecessor_row_value_formed in blast)
+  show ?thesis using first formed closed shape by simp
+qed
+
+theorem generation_predecessor_report_quotation_class:
+  "presentation_class
+    (composed_presentation generation_predecessor_report_presents (\<lambda>t p. complete_data_quoted_at (fst p) (snd p) t))
+    (\<lambda>z. generation_at_context (fst (fst z)) (snd (fst z)) \<and>
+      snd z=generation_predecessor_rows (fst (fst (fst z))) (fst (snd (fst (fst z)))) (snd (snd (fst (fst z)))))
+    (\<lambda>p. \<exists>t. (\<exists>z. generation_predecessor_report_presents z t) \<and> complete_data_quoted_at (fst p) (snd p) t)"
+  by (rule complete_quotation_presentation_class[OF generation_predecessor_report_presentation_class])
+    (use generation_predecessor_report_formed in blast)
+
+theorem generation_predecessor_report_total:
+  assumes source: "generation_at E u r G"
+  shows "\<exists>p q. generation_source_presents ((E,(u,r)),G) p \<and>
+    data_collection_presents generation_predecessor_row_presents (generation_predecessor_rows E u r) q \<and>
+    generation_predecessor_report_presents (((E,(u,r)),G),generation_predecessor_rows E u r) (Pair_Term p q) \<and>
+    complete_data_quoted_at (term_syntax (Pair_Term p q)) [] (Pair_Term p q)"
+proof -
+  obtain p where source_value: "generation_source_presents ((E,(u,r)),G) p"
+    using generation_source_presentation_total[OF source] by blast
+  have domain: "finite (generation_predecessor_rows E u r) \<and>
+      (\<forall>row\<in>generation_predecessor_rows E u r. generation_predecessor_row_formed row)"
+    using generation_predecessor_rows_complete(1)[OF source] generation_predecessor_rows_formed by blast
+  obtain q where rows: "data_collection_presents generation_predecessor_row_presents (generation_predecessor_rows E u r) q"
+    using generation_predecessor_collections.total[OF domain] by blast
+  have report: "generation_predecessor_report_presents
+      (((E,(u,r)),G),generation_predecessor_rows E u r) (Pair_Term p q)"
+    using source_value rows by (simp add: generation_predecessor_report_presents_def)
+  have formed: "term_formed (Pair_Term p q)" and closed: "self_contained_term (Pair_Term p q)"
+    using generation_predecessor_report_formed[OF report] by blast+
+  have quote: "complete_data_quoted_at (term_syntax (Pair_Term p q)) [] (Pair_Term p q)"
+    by (rule complete_data_quotation_total[OF formed closed])
+  show ?thesis using source_value rows report quote by blast
+qed
+
+corollary generation_predecessor_report_retention:
+  assumes source: "generation_source_presents ((E,(u,r)),G) p"
+    and retained: "generation_source_presents ((generation_source_environment E u r,(u,r)),G) p'"
+    and rows: "data_collection_presents generation_predecessor_row_presents L q"
+  shows "(\<exists>z. generation_predecessor_report_presents z (Pair_Term p' q)) \<longleftrightarrow>
+    (\<exists>z. generation_predecessor_report_presents z (Pair_Term p q))"
+proof -
+  have actual: "generation_at E u r G" using source by (simp add: generation_source_presents_def)
+  have site: "(u,r)\<in>generation_read_sites E {(u,r)}" using generation_read_sites_roots[of "{(u,r)}" E] by blast
+  have same: "generation_predecessor_rows (generation_source_environment E u r) u r=generation_predecessor_rows E u r"
+    using generation_source_environment_properties(7)[OF actual] site by blast
+  show ?thesis by (simp only: generation_predecessor_report_at_presentations[OF retained rows]
+    generation_predecessor_report_at_presentations[OF source rows] same)
+qed
+
+text \<open>
+  The source class retains its actual environment and selected site. The core
+  is recovered by the existing generation reading. Its covered image includes
+  every formed finite core, while the complete source remains recoverable from
+  each presentation. A core report is compatible only when it presents the
+  core actually read from that same source.
+
+  Predecessor rows retain the socket, citation endpoint, actual destination
+  use and address, and exact child core. Their domain is the complete native
+  socket domain. Each predecessor core occurs once. Every row in this native
+  collection recovers a real recursive reading at its stated site. The
+  request-edge equation preserves and reflects those actual sites. A different presentation of an
+  equal child core does not thereby become the cited destination.
+
+  The recovered core strictly decreases along every readable predecessor
+  edge. This proves well-foundedness on the complete set of recursively read
+  sites. The source restriction preserves all those rows, read sites, and
+  citation requests. It is closed, idempotent, and included in every retained
+  subenvironment that can still read the generation. Its artifact and binding
+  equations account for every retained item.
+
+  The row-report class uses products and complete collections, constrained by
+  that actual native relation. Every valid generation has such a report and
+  a complete quotation. All collection orders and member presentations remain
+  available. The explicit relation and retention equations establish joint
+  compatibility; separate class recovery is not substituted for those proofs.
+
+  These class and relation theorems do not add a native admission clause.
+  Native checking of the remaining recursive generation and higher protocol
+  relations still requires an ordinary program with its own exact contract.
+\<close>
+
+end
